append-sorted lemma

ulib/FStar.Seq.Sorted.fst
@@ -25,22 +25,30 @@ let rec sorted_pred_sorted_lemma #a f s =
     sorted_pred_sorted_lemma #a f (tail s)
   end
 
+let intro_sorted_pred (#a:eqtype) (f:tot_ord a) (s:seq a)
+  ($g:i:nat{i < length s} -> j:nat{j < length s} -> Lemma (requires (i <= j)) (ensures (f (index s i) (index s j))))
+  : Lemma (sorted_pred #a f s)
+= let aux (i j : k:nat{k < length s}) (p:squash (i <= j)) : GTot (squash (f (index s i) (index s j))) =
+    FStar.Squash.give_proof p ;
+    g i j ;
+    FStar.Squash.get_proof (f (index s i) (index s j))
+  in
+  FStar.Classical.forall_intro_2 (fun (i j:k:nat{k < length s}) ->
+    FStar.Classical.arrow_to_impl (aux i j) <: Lemma (i <= j ==> f (index s i) (index s j)))
+
 val sorted_pred_cons_lemma :
   #a:eqtype ->
   f:tot_ord a ->
   s:seq a{length s > 1} ->
   Lemma (requires (f (index s 0) (index s 1) /\ sorted_pred #a f (tail s))) (ensures (sorted_pred #a f s))
 let sorted_pred_cons_lemma #a f s =
-  let open FStar.Classical in
-  let aux (i j : k:nat{k < length s}) (p:squash (i <= j)) : GTot (squash (f (index s i) (index s j))) =
-    FStar.Squash.give_proof p ;
+  let aux (i j : k:nat{k < length s}) : Lemma (requires (i <= j)) (ensures (f (index s i) (index s j))) =
     if i = 0 then
       if j = 0 then ()
       else assert (f (index s 0) (index (tail s) 0) /\ f (index (tail s) 0) (index (tail s) (j-1)))
-    else assert (f (index (tail s) (i - 1)) (index (tail s) (j - 1))) ;
-    FStar.Squash.get_proof (f (index s i) (index s j))
+    else assert (f (index (tail s) (i - 1)) (index (tail s) (j - 1)))
   in
-  FStar.Classical.forall_intro_2 (fun (i j:k:nat{k < length s}) -> FStar.Classical.arrow_to_impl (aux i j) <: Lemma (i <= j ==> f (index s i) (index s j)))
+  intro_sorted_pred #a f s aux
 
 val sorted_sorted_pred_lemma :
   #a:eqtype ->
@@ -83,3 +91,23 @@ val sorted_split_lemma :
 let sorted_split_lemma #a f s i =
   sorted_slice_lemma #a f s 0 i ;
   sorted_slice_lemma #a f s i (length s)
+
+val sorted_pred_append_lemma :
+  #a:eqtype ->
+  f:tot_ord a ->
+  s1:seq a ->
+  s2:seq a ->
+  Lemma (requires (sorted_pred #a f s1 /\ sorted_pred #a f s2 /\ (length s1 > 0 /\ length s2 > 0 ==> f (last s1) (head s2))))
+    (ensures (sorted_pred #a f (append s1 s2)))
+let sorted_pred_append_lemma #a f s1 s2 =
+  let s = append s1 s2 in
+  let aux (i j:k:nat{k < length s}) : Lemma (requires (i <= j)) (ensures (f (index s i) (index s j))) =
+    if i < length s1 then
+      if j < length s1 then
+        assert (f (index s1 i) (index s1 j))
+      else
+        (assert (f (index s1 i) (last s1)) ; assert (f (head s2) (index s2 (j - length s1))))
+    else
+      (assert (j >= length s1) ; assert (f (index s2 (i - length s1)) (index s2 (j - length s1))))
+  in
+  intro_sorted_pred #a f s aux
